proved soundness of progress insensitive type system

theories/Secure/SecurityImpExc/SecurityImpTypesProgInsens.v
@@ -42,8 +42,6 @@ Import MonadNotation.
 Local Open Scope monad_scope.
 Local Open Scope string_scope.
 
-Instance sense_preorder_in : Preorder := sense_preorder.
-
 Notation label := sensitivity.
 
 Definition labelled_equiv  :=
@@ -132,10 +130,19 @@ Proof.
   red. intros. inv H; constructor; auto.
 Qed.
 
+(* You messed up the second case here 
+   it should be something like it either is left or 
+   it is above lexn 
+ *)
+
+Variant Rsense_unpriv (observer lexn : label) : unit + label -> Prop :=
+  | rup_inl : Rsense_unpriv observer lexn (inl tt)
+  | rup_priv_exc lpriv : ~ leq lpriv observer -> leq lpriv lexn -> Rsense_unpriv observer lexn (inr lpriv).
+
 Variant secure_throw_stmt_at_label (observer pc lexn : label) (s : stmt) : Prop :=
   | stsal_leq : leq pc observer -> label_state_pi_sec_eutt Γ observer (Rsense observer lexn )
                                                        (sem_throw_stmt s) (sem_throw_stmt s) -> secure_throw_stmt_at_label observer pc lexn s
-  | stsal_nleq : (~ leq pc observer) -> label_state_pi_sec_eutt Γ observer (fun sum _ => is_inl sum ) 
+  | stsal_nleq : (~ leq pc observer) -> label_state_pi_sec_eutt Γ observer (fun sum _ => Rsense_unpriv observer lexn sum ) 
                                                             (sem_throw_stmt s) (ret tt ) ->  secure_throw_stmt_at_label observer pc lexn s
   .
 (*maybe I can simplify the first return relation, I think some of those conditions are implied by a reasonable secure_stmt def 
@@ -148,49 +155,102 @@ Variant secure_throw_stmt_at_label (observer pc lexn : label) (s : stmt) : Prop 
 Definition secure_throw_stmt pc lexn s := forall observer, secure_throw_stmt_at_label observer pc lexn s.
 
 Lemma pi_sem_stmt_ret_aux:
-  forall (s2 : stmt) (observer : label) (σ3 σ4 : map),
+  forall (s1 s2 : stmt) (observer : label) (σ3 σ4 : map),
+    (forall σ1 σ2 : map,
+        labelled_equiv Γ observer σ1 σ2 ->
+        pi_eqit_secure sense_preorder priv_exc_io (product_rel (labelled_equiv Γ observer) top2)
+                       true true observer (sem_stmt s1 σ1) (Ret (σ2, tt))) ->
     (forall σ1 σ2 : map,
         labelled_equiv Γ observer σ1 σ2 ->
         pi_eqit_secure sense_preorder priv_exc_io (product_rel (labelled_equiv Γ observer) top2)
                        true true observer (sem_stmt s2 σ1) (Ret (σ2, tt))) ->
     labelled_equiv Γ observer σ3 σ4 ->
     pi_eqit_secure sense_preorder priv_exc_io (product_rel (labelled_equiv Γ observer) eq) true
-                   true observer (interp_state handle_imp (denote_stmt s2) σ3)
+                   true observer (interp_state handle_imp (denote_stmt s1) σ3)
                    (interp_state handle_imp (denote_stmt s2) σ4).
 Proof.
-  intros s2 observer σ3 σ4 Hσ Hs2.
+  intros s1 s2 observer σ3 σ4 Hσ Hs1 Hs2.
   eapply pi_eqit_secure_RR_imp with (RR1 := rcompose  (product_rel (labelled_equiv Γ observer) (@top2 unit unit)) (Basics.flip (product_rel (labelled_equiv Γ observer) top2))).
   { intros [σ5 [] ] [σ6 [] ] Hr. inv Hr. inv REL1. inv REL2. split; auto.
     destruct r2 as [σ7 [] ]. etransitivity; eauto. symmetry. auto.
   }
   eapply pi_eqit_secure_trans_ret; eauto. 
-  apply pi_eqit_secure_sym. apply Hσ. reflexivity.
+  apply pi_eqit_secure_sym. eapply Hs1. reflexivity.
 Qed.
 
 Lemma pi_sem_throw_stmt_ret_aux:
-  forall (lexn : label) (s2 : stmt) (observer : label) (σ3 σ4 : map),
+  forall (lexn: label) (s1 s2 : stmt) (observer : label) (σ3 σ4 : map),
     (forall σ1 σ2 : map,
         labelled_equiv Γ observer σ1 σ2 ->
         pi_eqit_secure sense_preorder priv_exc_io
                        (product_rel (labelled_equiv Γ observer)
-                                    (fun (sum : unit + label) (_ : unit) => is_inl sum)) true true observer
+                                    (fun (sum : unit + label) (_ : unit) => Rsense_unpriv observer lexn sum)) true true observer
+                       (sem_throw_stmt s1 σ1) (Ret (σ2, tt))) ->
+    (forall σ1 σ2 : map,
+        labelled_equiv Γ observer σ1 σ2 ->
+        pi_eqit_secure sense_preorder priv_exc_io
+                       (product_rel (labelled_equiv Γ observer)
+                                    (fun (sum : unit + label) (_ : unit) => Rsense_unpriv observer lexn sum)) true true observer
                        (sem_throw_stmt s2 σ1) (Ret (σ2, tt))) ->
     labelled_equiv Γ observer σ3 σ4 ->
     pi_eqit_secure sense_preorder priv_exc_io
                    (product_rel (labelled_equiv Γ observer) (Rsense observer lexn)) true true
-                   observer (interp_state handle_imp (throw_prefix (denote_stmt s2)) σ3)
+                   observer (interp_state handle_imp (throw_prefix (denote_stmt s1)) σ3)
                    (interp_state handle_imp (throw_prefix (denote_stmt s2)) σ4).
 Proof.
-  intros lexn s2 observer σ3 σ4 Hσ H4.
-  set (product_rel (labelled_equiv Γ observer) (fun (sum : unit + label) ( _ : unit) => is_inl sum ) ) as HR.
+  intros lexn s1 s2 observer σ3 σ4 Hs1 Hs2 Hσ.
+  set (product_rel (labelled_equiv Γ observer) (fun (sum : unit + label) ( _ : unit) => Rsense_unpriv observer lexn sum ) ) as HR.
   eapply pi_eqit_secure_RR_imp with (RR1 := rcompose HR (Basics.flip HR) ).
   { unfold HR. intros [σ5 r1] [σ6 r2] Hr. inv Hr. inv REL1. inv REL2.
-    inv H0. inv H2. cbn in H3. cbn in H0. subst.
+    inv H0. inv H2. cbn in H3. cbn in H0. subst. 
     destruct r0 as [σ7 [] ]. split. etransitivity; eauto. symmetry. auto.
-    cbn. destruct a. destruct a0. constructor. }
+    constructor. cbn in H5. subst. destruct r0 as [σ7 [] ]. split. etransitivity; eauto. symmetry. auto.
+    cbn in H3. subst. constructor; auto. cbn in H5. cbn in H2.
+    subst. destruct r0. split. etransitivity; eauto. symmetry. auto.
+    cbn. inv H2. constructor; auto. constructor; auto.
+  }
   eapply pi_eqit_secure_trans_ret; eauto. apply pi_eqit_secure_sym.
-  eapply Hσ. reflexivity.
+  eapply Hs2. reflexivity.
 Qed.
+
+Lemma lower_lexn_sound lexn1 lexn2 t1 t2 observer :
+  leq lexn1 lexn2 ->
+  pi_eqit_secure sense_preorder priv_exc_io
+                 (product_rel (labelled_equiv Γ observer) (Rsense observer lexn1)) true true
+                 observer t1 t2 ->
+  pi_eqit_secure sense_preorder priv_exc_io
+                 (product_rel (labelled_equiv Γ observer) (Rsense observer lexn2)) true true
+                 observer t1 t2.
+Proof.
+  intros. eapply pi_eqit_secure_RR_imp; try apply H0.
+  intros [σ1 r1] [σ2 r2] [Hσ Hr]. inv Hr.
+  all : split; auto.
+  - cbn in *; subst; constructor.
+  - cbn in H3; cbn in H4; subst. constructor; auto.
+    all : eapply leq_sense_trans; eauto.
+  - cbn in H3; cbn in H4; subst. constructor; auto.
+    eapply leq_sense_trans; eauto.
+  - cbn in H3; cbn in H4; subst. constructor; auto.
+    eapply leq_sense_trans; eauto.
+Qed.
+
+Lemma lower_lexn_sound' lexn1 lexn2 t1 t2 observer :
+  leq lexn1 lexn2 ->
+  pi_eqit_secure sense_preorder priv_exc_io
+                 (product_rel (labelled_equiv Γ observer) (fun (sum : unit + label) (_ : unit) => Rsense_unpriv observer lexn1 sum)) true true
+                 observer t1 t2 ->
+  pi_eqit_secure sense_preorder priv_exc_io
+                 (product_rel (labelled_equiv Γ observer) (fun (sum : unit + label) (_ : unit) => Rsense_unpriv observer lexn2 sum)) true true
+                 observer t1 t2.
+Proof.
+  intros. eapply pi_eqit_secure_RR_imp; try apply H0.
+  intros [σ1 r1] [σ2 [] ] [Hσ Hr]; inv Hr.
+  - cbn in H1; subst. split; auto. constructor.
+  - cbn in H3. subst. split; auto.
+    constructor; auto. eapply leq_sense_trans; eauto.
+Qed.
+
+
 
 Lemma seq_well_typed_correct pc lexn1 lexn2 s1 s2 :
   secure_stmt pc lexn1 s1 -> secure_stmt (join pc lexn1) lexn2 s2 ->
@@ -233,6 +293,7 @@ Proof.
         try eapply leq_sense_trans; eauto; apply leq_sense_join_r.
       * cbn in H4. cbn.
         do 2 red in H4. cbn in Hσ'.
+        eapply lower_lexn_sound. apply leq_sense_join_r.
         eapply pi_sem_throw_stmt_ret_aux; eauto.
     + setoid_rewrite interp_state_ret. apply pi_eqit_secure_ret.
       split; auto; constructor; eapply leq_sense_trans; eauto.
@@ -248,9 +309,11 @@ Proof.
         rewrite H7. rewrite <- bind_ret_r.
         eapply pi_eqit_secure_bind; eauto.
         intros [σ5 r3] [σ6 r4] [Hσ'' Hr']; inv Hr'.
-        cbn in H8. rewrite <- H8. destruct a. apply pi_eqit_secure_ret.
-        split; auto. constructor; auto. eapply leq_sense_trans; eauto.
-        apply leq_sense_join_l.
+        -- cbn in H8. subst. apply pi_eqit_secure_ret. split; auto.
+           constructor; auto. eapply leq_sense_trans; eauto. apply leq_sense_join_l.
+        -- cbn in H10. subst. apply pi_eqit_secure_ret. split; auto.
+           constructor; auto. eapply leq_sense_trans; eauto. apply leq_sense_join_r.
+           eapply leq_sense_trans; eauto. apply leq_sense_join_l.
     + specialize (Hs2 observer). inv Hs2; eauto.
       * exfalso. apply H2. eapply leq_sense_trans; eauto.
         eapply leq_sense_trans; eauto. apply leq_sense_join_r.
@@ -262,17 +325,21 @@ Proof.
         setoid_rewrite <- bind_ret_r at 4.
         apply pi_eqit_secure_sym. symmetry in Hσ'. eapply pi_eqit_secure_bind; eauto.
         intros [σ5 r3] [σ6 [] ] [Hσ'' Hr']; inv Hr'.
-        destruct a. cbn in H8. subst. apply pi_eqit_secure_ret.
-        split; auto. symmetry. auto. constructor; auto.
-        eapply leq_sense_trans; eauto. apply leq_sense_join_l.
+        -- cbn in H8. subst. apply pi_eqit_secure_ret. split; auto. symmetry. auto.
+           constructor; auto. eapply leq_sense_trans; eauto. apply leq_sense_join_l.
+        -- cbn in H10. subst. apply pi_eqit_secure_ret. split; auto. symmetry. auto.
+           constructor. eapply leq_sense_trans; eauto. apply leq_sense_join_l.
+           eapply leq_sense_trans; eauto. apply leq_sense_join_r.
   - right; auto. intros σ1 σ2 Hσ. unfold sem_throw_stmt, interp_imp.
     cbn. setoid_rewrite throw_prefix_bind. setoid_rewrite interp_state_bind.
     cbn in H0. rewrite <- bind_ret_r with (s := Ret (σ2, tt) ).
     eapply pi_eqit_secure_bind; eauto. intros [σ3 r1] [σ4 [] ] [Hσ' Hr]. inv Hr.
-    destruct a. cbn. cbn in H1. subst.
-    specialize (Hs2 observer). inv Hs2.
-    + exfalso. apply H. eapply leq_sense_trans; eauto. apply leq_sense_join_l.
-    + cbn in H2. eauto.
+    -- cbn in H1. subst. cbn. specialize (Hs2 observer). inv Hs2.
+       ++ exfalso. apply H. eapply leq_sense_trans; eauto. apply leq_sense_join_l.
+       ++ cbn in H2. eapply lower_lexn_sound'; eauto. apply leq_sense_join_r.
+    -- cbn in H3. subst. cbn.  setoid_rewrite interp_state_ret.
+       apply pi_eqit_secure_ret. split; auto. constructor; auto.
+       eapply leq_sense_trans; eauto. apply leq_sense_join_l.
 Qed.
 
 Lemma try_catch_well_typed_correct pc lexn1 lexn2 s1 s2 :
@@ -313,8 +380,10 @@ Proof.
     setoid_rewrite interp_state_bind. cbn in H2.
     eapply pi_eqit_secure_bind; eauto.
     intros [σ3 r1] [σ4 [] ] [Hσ' Hr]; inv Hr.
-    destruct a. simpl. setoid_rewrite interp_state_ret.
-    apply pi_eqit_secure_ret. split; cbv; auto.
+    + tau_steps. apply pi_eqit_secure_ret. split; auto. cbv. auto.
+    + specialize (Hs2 observer). inv Hs2; eauto.
+      * exfalso. apply H. eapply leq_sense_trans; eauto. apply leq_sense_join_l.
+      * cbn in H8. eauto.
 Qed.
 
 Lemma try_catch_well_typed_correct' pc lexn1 lexn2 s1 s2 :
@@ -346,8 +415,11 @@ Proof.
         |- pi_eqit_secure _ _ _ _ _ _ _ ?t => assert (t ≈ ITree.bind (Ret (σ3, tt) ) (fun '(σ, x) => Ret (σ, inl x) ) ) end.
         rewrite bind_ret_l. reflexivity. rewrite H9.
         rewrite <- bind_ret_r. symmetry in Hσ'. eapply pi_eqit_secure_bind; eauto.
-        intros [σ5 r] [σ6 [] ] Hr. inv Hr. inv H11. destruct a. cbn in H12. subst.
-        apply pi_eqit_secure_ret. split. symmetry; auto. constructor.
+        intros [σ5 r] [σ6 [] ] Hr. inv Hr. inv H11. 
+        -- apply pi_eqit_secure_ret. split. symmetry. auto. cbn in H12. subst.
+           constructor.
+        -- cbn in H14. subst. apply pi_eqit_secure_ret. split. symmetry. auto.
+           constructor; auto.
     + specialize (Hs2 observer). inv Hs2; eauto.
       * exfalso. apply H4. eapply leq_sense_trans; eauto.
         eapply leq_sense_trans; eauto. apply leq_sense_join_r.
@@ -356,8 +428,11 @@ Proof.
         |- pi_eqit_secure _ _ _ _ _ _ _ ?t => assert (t ≈ ITree.bind (Ret (σ4, tt) ) (fun '(σ, x) => Ret (σ, inl x) ) ) end.
         rewrite bind_ret_l. reflexivity. rewrite H9. cbn in H8.
         rewrite <- bind_ret_r. eapply pi_eqit_secure_bind; eauto.
-        intros [σ5 r] [σ6 [] ] Hr. inv Hr. inv H11. destruct a. cbn in H12. subst.
-        apply pi_eqit_secure_ret. split; auto. constructor.
+        intros [σ5 r] [σ6 [] ] Hr. inv Hr. inv H11. 
+        -- cbn in H12. subst. apply pi_eqit_secure_ret. constructor.
+           auto. constructor.
+        -- cbn in H14. subst. apply pi_eqit_secure_ret. split; auto.
+           constructor; auto.
   - right; auto. unfold sem_throw_stmt, interp_imp. cbn. do 2 red.
     intros σ1 σ2 Hσ. rewrite throw_prefix_of_try_catch.
     rewrite try_catch_to_throw_prefix.
@@ -367,9 +442,13 @@ Proof.
     cbn in H2.
     eapply pi_eqit_secure_bind; eauto.
     intros [σ3 r1] [σ4 r2] [Hσ' Hr]; inv Hr.
-    rewrite throw_prefix_ret, interp_state_ret, bind_ret_l. cbn.
-    rewrite interp_state_ret. apply pi_eqit_secure_ret. split; auto.
-    constructor.
+    + rewrite throw_prefix_ret, interp_state_ret, bind_ret_l. cbn.
+      rewrite interp_state_ret. apply pi_eqit_secure_ret. split; auto.
+      constructor.
+    + specialize (Hs2 observer). inv Hs2; eauto.
+      * exfalso. apply H. eapply leq_sense_trans; eauto. apply leq_sense_join_l.
+      * cbn in H7. setoid_rewrite interp_state_ret. rewrite bind_ret_l.
+        cbn. destruct r2. eauto.
 Qed.
 
 Lemma pi_eqit_secure_while_ret_aux:
@@ -400,8 +479,46 @@ Proof.
     apply pi_eqit_secure_ret. constructor. split; auto.
 Qed.
 
-Lemma while_typed_correct e le pc lexn s :
-  secure_expr le e -> secure_stmt (join pc le) lexn s -> secure_stmt pc lexn (While e s).
+Lemma pi_eqit_secure_while_ret_throw_aux:
+  forall (e : expr) (s : stmt) (observer lexn : label),
+    label_state_pi_sec_eutt Γ observer (fun (sum : unit + label) (_ : unit) => Rsense_unpriv observer lexn sum)
+                            (sem_throw_stmt s) (ret tt) ->
+    forall σ1 σ2 : map,
+      labelled_equiv Γ observer σ1 σ2 -> 
+      pi_eqit_secure sense_preorder priv_exc_io
+                     (product_rel (labelled_equiv Γ observer)
+                                  (fun (sum : unit + label) (_ : unit) => Rsense_unpriv observer lexn sum)) true true observer
+                     (sem_throw_stmt (While e s) σ1) (Ret (σ2, tt)).
+Proof.
+  intros e s observer lexn H0 σ1 σ2 Hσ.
+  unfold sem_throw_stmt, interp_imp.
+  cbn. setoid_rewrite throw_prefix_iter.
+  specialize (@interp_state_iter') as Hisi. red in Hisi. setoid_rewrite Hisi.
+  apply pi_eqit_secure_iter_ret with (Rinv := product_rel (labelled_equiv Γ observer) eq).
+  2 : split; auto.
+  intros [σ3 [] ] [Hσ3 _ ]. cbn. cbn in Hσ3. setoid_rewrite throw_prefix_bind.
+  repeat setoid_rewrite interp_state_bind. repeat rewrite bind_bind.
+  rewrite throw_prefix_denote_expr. rewrite interp_state_bind, bind_bind.
+  specialize (expr_only_ret' e σ3) as [n Hn]. setoid_rewrite Hn.
+  rewrite bind_ret_l, interp_state_ret, bind_ret_l. cbn.
+  destruct n.
+  + rewrite throw_prefix_ret, interp_state_ret, bind_ret_l. cbn.
+    rewrite interp_state_ret. rewrite bind_ret_l. cbn.
+    apply pi_eqit_secure_ret. constructor. split; auto.
+    constructor.
+  + rewrite throw_prefix_bind. rewrite interp_state_bind. rewrite bind_bind.
+    rewrite <- bind_ret_r with (s0 := Ret (σ2, tt) ).
+    cbn in H0.
+    eapply pi_eqit_secure_bind; eauto.
+    intros [σ4 r1] [σ5 r2] [Hσ' Hr]; inv Hr.
+    * cbn in H. subst. tau_steps. apply pi_eqit_secure_ret.
+      constructor; auto. split; auto. destruct r2. auto.
+    * cbn in H2. subst. tau_steps.
+      apply pi_eqit_secure_ret. constructor. split; auto. constructor; auto.
+Qed.
+
+Lemma while_well_typed_correct e le pc lexn s :
+  secure_expr le e -> secure_stmt (join pc (join le lexn)) lexn s -> secure_stmt pc lexn (While e s).
 Proof.
   intros He Hs observer.
   specialize (He observer). specialize (Hs observer).
@@ -423,11 +540,15 @@ Proof.
       intros [σ5 [] ] [σ6 [] ] [Hσ'' _ ]. setoid_rewrite interp_state_ret.
       setoid_rewrite bind_ret_l. cbn. apply pi_eqit_secure_ret.
       constructor; auto.
-  - exfalso. apply H1. eapply leq_sense_trans; eauto. apply leq_sense_join_r.
-  - right. intro. apply H. 
-    (* come up with a lemma for this *)
-    destruct pc; destruct le; destruct observer; cbv; auto.
-    do 2 red. intros. cbn. eapply pi_eqit_secure_while_ret_aux; eauto.
+  - exfalso. apply H1. 
+    eapply leq_sense_trans with (l2 := join le lexn); eauto. 
+    apply leq_sense_join_l.
+    eapply leq_sense_trans; try apply leq_sense_join_r. eauto.
+  - case_leq pc observer.
+    + left; auto. intros σ1 σ2 Hσ.
+      specialize (pi_eqit_secure_while_ret_aux e s observer H0) as Hwhile.
+      eapply pi_sem_stmt_ret_aux; eauto.
+    + right; auto. cbn. do 2 red. intros. eapply pi_eqit_secure_while_ret_aux; eauto.
   - case_leq pc observer.
     + left; auto. intros σ1 σ2 Hσ.
       specialize (pi_eqit_secure_while_ret_aux e s observer H0) as Hwhile.
@@ -436,8 +557,9 @@ Proof.
 Qed.
 
 
-Lemma while_typed_correct' e le pc lexn s : 
-  secure_expr le e -> secure_throw_stmt (join pc le) lexn s -> secure_throw_stmt pc lexn (While e s).
+
+Lemma while_well_typed_correct' e le pc lexn s : 
+  secure_expr le e -> secure_throw_stmt (join pc (join le lexn)) lexn s -> secure_throw_stmt pc lexn (While e s).
 Proof.
   intros He Hs observer.
   specialize (He observer). specialize (Hs observer).
@@ -464,25 +586,396 @@ Proof.
         apply pi_eqit_secure_ret. constructor. split; auto.
       * tau_steps. apply pi_eqit_secure_ret. constructor. split; auto.
         constructor; auto.
-      * tau_steps. cbn in Hσ'. cbn in Hσ''. cbn in Hσ'''. admit.
-      * tau_steps. admit.
+      * exfalso. apply H4.
+        eapply leq_sense_trans; eauto.
+        eapply leq_sense_trans; try apply H.
+        eapply leq_sense_trans with (l2 := join le lexn); eauto.
+        apply leq_sense_join_r. apply leq_sense_join_r.
+      * exfalso.  apply H4.
+        eapply leq_sense_trans; eauto.
+        eapply leq_sense_trans; try apply H.
+        eapply leq_sense_trans with (l2 := join le lexn); eauto.
+        apply leq_sense_join_r. apply leq_sense_join_r.
+  - exfalso. apply H1. eapply leq_sense_trans; eauto. 
+    eapply leq_sense_trans with (l2 := join le lexn).  
+    apply leq_sense_join_l. apply leq_sense_join_r.
+  - case_leq pc observer.
+    + left; auto. intros σ1 σ2 Hσ.
+      specialize (pi_eqit_secure_while_ret_throw_aux e s observer) as Hwhile.
+      eapply pi_sem_throw_stmt_ret_aux; eauto.
+    + right; auto. cbn. intros σ1 σ2 Hσ.
+      eapply pi_eqit_secure_while_ret_throw_aux; eauto.
+  - case_leq pc observer.
+    + left; auto. intros σ1 σ2 Hσ.
+      specialize (pi_eqit_secure_while_ret_throw_aux e s observer) as Hwhile.
+      eapply pi_sem_throw_stmt_ret_aux; eauto.
+    + right; auto. cbn. intros σ1 σ2 Hσ.
+      eapply pi_eqit_secure_while_ret_throw_aux; eauto.
+Qed.
 
-  - exfalso. apply H1. eapply leq_sense_trans; eauto. apply leq_sense_join_r.
-  - right. intro. apply H.
-    destruct pc; destruct le; destruct observer; cbv; auto.
-    (* need a lemma to relate iter to ret *) admit.
-Abort. 
+Lemma if_well_typed_correct e le pc lexn1 lexn2 s1 s2 :
+  secure_expr le e -> secure_stmt (join pc le) lexn1 s1 ->
+  secure_stmt (join pc le) lexn2 s2 ->
+  secure_stmt pc (join lexn1 lexn2) (If e s1 s2).
+Proof.
+  intros He Hs1 Hs2 observer.
+  specialize (Hs1 observer). specialize (Hs2 observer).
+  specialize (He observer).
+  inv Hs1; inv Hs2; inv He; try contradiction.
+  - left; auto. eapply leq_sense_trans with (l2 := join pc le);  eauto.
+    apply leq_sense_join_l.
+    intros σ1 σ2 Hσ. unfold sem_stmt, interp_imp.
+    cbn. setoid_rewrite interp_state_bind.
+    eapply pi_eqit_secure_bind; eauto. 
+    intros [σ3 v1] [σ4 v2] [Hσ' Hv]; cbn in Hv; subst.
+    destruct v2; cbn; eauto.
+  - exfalso. apply H3. eapply leq_sense_trans; eauto.
+    apply leq_sense_join_r.
+  - right. intro. apply H. destruct pc; destruct le; auto.
+    intros σ1 σ2 Hσ. unfold sem_stmt, interp_imp. cbn.
+    setoid_rewrite interp_state_bind.
+    specialize (expr_only_ret' e σ1) as [n Hn]. setoid_rewrite Hn.
+    rewrite bind_ret_l. destruct n; cbn in *; eauto.
+  - case_leq pc observer.
+    + left; auto. intros σ1 σ2 Hσ. unfold sem_stmt, interp_imp. cbn.
+      setoid_rewrite interp_state_bind.
+      specialize (expr_only_ret' e σ1) as [n1 Hn1]. setoid_rewrite Hn1.
+      specialize (expr_only_ret' e σ2) as [n2 Hn2]. setoid_rewrite Hn2.
+      setoid_rewrite bind_ret_l.
+      destruct n1; destruct n2; cbn;
+        eapply pi_sem_stmt_ret_aux; eauto.
+    + right; auto.
+      intros σ1 σ2 Hσ. unfold sem_stmt, interp_imp. cbn.
+      setoid_rewrite interp_state_bind.
+      specialize (expr_only_ret' e σ1) as [n1 Hn1]. setoid_rewrite Hn1.
+      rewrite bind_ret_l. destruct n1; cbn in *; eauto.
+Qed.
 
-Inductive well_typed_expr : sensitivity -> expr -> Prop :=
-  | wte_lit l n : well_typed_expr l (Lit n)
-  | wte_var x l : leq (Γ x) l -> well_typed_expr l (Var x)
-  | wte_plus l1 l2 e1 e2 : well_typed_expr l1 e1 -> well_typed_expr l2 e2 ->
-                           well_typed_expr (join l1 l2) (Plus e1 e2)
-  | wte_min l1 l2 e1 e2 : well_typed_expr l1 e1 -> well_typed_expr l2 e2 ->
-                           well_typed_expr (join l1 l2) (Minus e1 e2)
-  | wte_mult l1 l2 e1 e2 : well_typed_expr l1 e1 -> well_typed_expr l2 e2 ->
-                           well_typed_expr (join l1 l2) (Mult e1 e2)
-.
+Lemma if_well_typed_correct' e le pc lexn1 lexn2 s1 s2 :
+  secure_expr le e -> secure_throw_stmt (join pc le) lexn1 s1 ->
+  secure_throw_stmt (join pc le) lexn2 s2 ->
+  secure_throw_stmt pc (join lexn1 lexn2) (If e s1 s2).
+Proof.
+  intros He Hs1 Hs2 observer.
+  specialize (Hs1 observer). specialize (Hs2 observer).
+  specialize (He observer).
+  inv Hs1; inv Hs2; inv He; try contradiction.
+  - left; auto. eapply leq_sense_trans with (l2 := join pc le);  eauto.
+    apply leq_sense_join_l.
+    unfold sem_throw_stmt, interp_imp. intros σ1 σ2 Hσ.
+    cbn. setoid_rewrite throw_prefix_bind.
+    rewrite throw_prefix_denote_expr.
+    repeat setoid_rewrite interp_state_bind.
+    repeat setoid_rewrite bind_bind.
+    eapply pi_eqit_secure_bind; eauto.
+    intros [σ3 v1] [σ4 v2] [Hσ' Hv]; cbn in Hv; subst.
+    setoid_rewrite interp_state_ret. setoid_rewrite bind_ret_l.
+    cbn. destruct v2; eauto. 
+    eapply lower_lexn_sound; eauto. apply leq_sense_join_r.
+    eapply lower_lexn_sound; eauto. apply leq_sense_join_l.
+  - exfalso. apply H3. eapply leq_sense_trans; eauto. apply leq_sense_join_r.
+  - right. intro. apply H. destruct pc; destruct le; auto.
+    intros σ1 σ2 Hσ. unfold sem_throw_stmt, interp_imp.
+    cbn. setoid_rewrite throw_prefix_bind.
+    setoid_rewrite throw_prefix_denote_expr.
+    repeat rewrite interp_state_bind. repeat rewrite bind_bind.
+    specialize (expr_only_ret' e σ1) as [n1 Hn1]. setoid_rewrite Hn1.
+    rewrite bind_ret_l. rewrite interp_state_ret, bind_ret_l.
+    cbn.
+    destruct n1; cbn in *; eapply lower_lexn_sound'; eauto.
+    apply leq_sense_join_r. apply leq_sense_join_l.
+  - case_leq pc observer.
+    + left; auto. intros σ1 σ2 Hσ. unfold sem_throw_stmt, interp_imp.
+      cbn. setoid_rewrite throw_prefix_bind. setoid_rewrite interp_state_bind.
+      setoid_rewrite throw_prefix_denote_expr. setoid_rewrite interp_state_bind.
+      repeat rewrite bind_bind. 
+      specialize (expr_only_ret' e σ1) as [n1 Hn1]. setoid_rewrite Hn1.
+      specialize (expr_only_ret' e σ2) as [n2 Hn2]. setoid_rewrite Hn2.
+      setoid_rewrite bind_ret_l. setoid_rewrite interp_state_ret.
+      setoid_rewrite bind_ret_l. cbn. 
+      assert (label_state_pi_sec_eutt Γ observer
+         (fun (sum : unit + label) (_ : unit) => Rsense_unpriv observer (join lexn1 lexn2) sum)
+         (sem_throw_stmt s1) (ret tt)).
+      { do 2 red. intros. eapply lower_lexn_sound'; eauto. apply leq_sense_join_l. }
+      assert (label_state_pi_sec_eutt Γ observer
+         (fun (sum : unit + label) (_ : unit) => Rsense_unpriv observer (join lexn1 lexn2) sum)
+         (sem_throw_stmt s2) (ret tt)).
+      { do 2 red. intros. eapply lower_lexn_sound'; eauto. apply leq_sense_join_r. }
+      destruct n1; destruct n2; cbn in *; try eapply pi_sem_throw_stmt_ret_aux; eauto.
+   + right; auto. 
+     intros σ1 σ2 Hσ. unfold sem_throw_stmt, interp_imp. cbn.
+     setoid_rewrite throw_prefix_bind. setoid_rewrite throw_prefix_denote_expr.
+     repeat rewrite interp_state_bind. repeat rewrite bind_bind.
+     specialize (expr_only_ret' e σ1) as [n1 Hn1]. setoid_rewrite Hn1.
+     rewrite bind_ret_l. rewrite interp_state_ret, bind_ret_l. cbn.
+     destruct n1; try eapply lower_lexn_sound'; cbn in *; eauto.
+     apply leq_sense_join_r. apply leq_sense_join_l.
+Qed.
+
+Lemma secure_expr_upward_close
+     : forall (e : expr) (l1 l2 : L),
+       leq l1 l2 -> secure_expr l1 e -> secure_expr l2 e.
+Proof.
+  intros e l1 l2 Hl He observer.
+  specialize (He observer). inv He.
+  - case_leq l2 observer.
+    + left; auto.
+    + right; auto.
+      exists 0. do 2 red. intros. cbn.
+      specialize (expr_only_ret' e σ1) as [n Hn]. rewrite Hn.
+      apply pi_eqit_secure_ret. split; auto. cbv. auto.
+  - case_leq l2 observer.
+    + left; auto. exfalso. apply H. eapply leq_sense_trans; eauto.
+    + right; auto.
+Qed.
+
+Lemma assign_well_typed_correct e le pc x : 
+  secure_expr le e -> leq (join le pc) (Γ x) ->
+  secure_stmt pc Public (Assign x e).
+Proof.
+  intros Hle Hx. 
+  assert (Hpc : leq pc (Γ x) ).
+  { eapply leq_sense_trans; eauto. apply leq_sense_join_r. }
+  assert (Hl : leq le (Γ x) ).
+  { eapply leq_sense_trans; try apply H5. apply leq_sense_join_l. eauto. }
+  assert (He : secure_expr (Γ x) e ).
+  { eapply secure_expr_upward_close with (l2:= Γ x); eauto. }
+  intros observer.
+  specialize ( He observer). inv He.
+  - left. eapply leq_sense_trans; eauto.
+    do 2 red in H0. do 2 red. intros. unfold sem_stmt.
+    cbn. unfold interp_imp. 
+    setoid_rewrite interp_state_bind. eapply pi_eqit_secure_bind; eauto.
+    intros [σ3 v1] [σ4 v2] [Hσ Hv]; cbn in Hv; subst.
+    setoid_rewrite interp_state_trigger. cbn. apply pi_eqit_secure_ret.
+    split; auto. cbn. eapply update_labelled_equiv_visible; auto.
+  - case_leq pc observer.
+    + left; auto. 
+      destruct H0 as [n Hn]. unfold sem_stmt.
+      cbn. unfold interp_imp. do 2 red. intros. setoid_rewrite interp_state_bind.
+      specialize (expr_only_ret' e σ1) as [n1 Hn1]. setoid_rewrite Hn1.
+      specialize (expr_only_ret' e σ2) as [n2 Hn2]. setoid_rewrite Hn2.
+      setoid_rewrite bind_ret_l. cbn. setoid_rewrite interp_state_trigger.
+      cbn. apply pi_eqit_secure_ret. split; auto.
+      cbn. apply update_labelled_equiv_invisible; auto. symmetry.
+      apply update_labelled_equiv_invisible; auto. symmetry; auto. 
+    + right; auto.
+      unfold sem_stmt, interp_imp. cbn. intros σ1 σ2 Hσ.
+      setoid_rewrite interp_state_bind.
+      specialize (expr_only_ret' e σ1) as [n1 Hn1]. setoid_rewrite Hn1.
+      rewrite bind_ret_l. setoid_rewrite interp_state_trigger.
+      cbn. apply pi_eqit_secure_ret.
+      split. 2 : cbv; auto. cbn. apply update_labelled_equiv_invisible; auto.
+Qed.
+
+Lemma assign_well_typed_correct' e le pc x : 
+  secure_expr le e -> leq (join le pc) (Γ x) ->
+  secure_throw_stmt pc Public (Assign x e).
+Proof.
+  intros Hle Hx. 
+  assert (Hpc : leq pc (Γ x) ).
+  { eapply leq_sense_trans; eauto. apply leq_sense_join_r. }
+  assert (Hl : leq le (Γ x) ).
+  { eapply leq_sense_trans; try apply H5. apply leq_sense_join_l. eauto. }
+  assert (He : secure_expr (Γ x) e ).
+  { eapply secure_expr_upward_close with (l2:= Γ x); eauto. }
+  intros observer.
+  specialize ( He observer). inv He.
+  - left. eapply leq_sense_trans; eauto.
+    do 2 red in H0. do 2 red. intros. unfold sem_throw_stmt.
+    cbn. unfold interp_imp. setoid_rewrite throw_prefix_bind.
+    setoid_rewrite throw_prefix_denote_expr.
+    setoid_rewrite interp_state_bind. 
+    setoid_rewrite interp_state_bind. repeat rewrite bind_bind.
+    eapply pi_eqit_secure_bind; eauto.
+    intros [σ3 v1] [σ4 v2] [Hσ Hv]; cbn in Hv; subst.
+    setoid_rewrite interp_state_ret. setoid_rewrite bind_ret_l. cbn.
+    setoid_rewrite throw_prefix_ev.
+    setoid_rewrite interp_state_vis. cbn. 
+    setoid_rewrite bind_ret_l. tau_steps.
+    apply pi_eqit_secure_ret.
+    split; auto. cbn. eapply update_labelled_equiv_visible; auto.
+    constructor.
+  - case_leq pc observer.
+    + left; auto. 
+      destruct H0 as [n Hn]. unfold sem_throw_stmt.
+      cbn. unfold interp_imp. do 2 red. intros. 
+      setoid_rewrite throw_prefix_bind. setoid_rewrite throw_prefix_denote_expr.
+      repeat setoid_rewrite interp_state_bind.
+      specialize (expr_only_ret' e σ1) as [n1 Hn1]. setoid_rewrite Hn1.
+      specialize (expr_only_ret' e σ2) as [n2 Hn2]. setoid_rewrite Hn2.
+      repeat rewrite bind_ret_l. tau_steps.
+      apply pi_eqit_secure_ret. split; auto.
+      cbn. apply update_labelled_equiv_invisible; auto. symmetry.
+      apply update_labelled_equiv_invisible; auto. symmetry; auto. 
+      constructor.
+    + right; auto.
+      unfold sem_throw_stmt, interp_imp. cbn. intros σ1 σ2 Hσ.
+      setoid_rewrite throw_prefix_bind. 
+      setoid_rewrite interp_state_bind. rewrite throw_prefix_denote_expr.
+      setoid_rewrite interp_state_bind.
+      specialize (expr_only_ret' e σ1) as [n1 Hn1]. setoid_rewrite Hn1.
+      tau_steps.
+      apply pi_eqit_secure_ret.
+      split. 2 : constructor. cbn. apply update_labelled_equiv_invisible; auto.
+Qed.
+
+Lemma print_well_typed_correct pc le lp e :
+  secure_expr le e -> leq (join le pc) lp ->
+  secure_stmt pc Public (Output lp e).
+Proof.
+  intros He0 Hle1.
+  assert (Hle : leq le lp).
+  { eapply leq_sense_trans; eauto. apply leq_sense_join_l. }
+  assert (Hpc : leq pc lp).
+  { eapply leq_sense_trans; try apply H5. apply leq_sense_join_r; eauto. eauto.  }
+  assert (He : secure_expr lp e ).
+  { eapply secure_expr_upward_close with (l1 := le); eauto. }
+  intros observer. specialize (He observer).
+  inv He.
+  - left. eapply leq_sense_trans; eauto.
+    unfold sem_stmt, interp_imp. intros σ1 σ2 Hσ.
+    cbn. setoid_rewrite interp_state_bind.
+    eapply pi_eqit_secure_bind; eauto.
+    intros [σ3 v1] [σ4 v4] [Hσ' Hv]; cbn in Hv; subst.
+    cbn. setoid_rewrite interp_state_trigger. cbn.
+    setoid_rewrite bind_trigger. apply pi_eqit_secure_pub_vis.
+    auto. intros []. apply pi_eqit_secure_ret. split; auto.
+  - case_leq pc observer.
+    + left; auto. unfold sem_stmt, interp_imp. intros σ1 σ2 Hσ.
+      cbn. setoid_rewrite interp_state_bind.
+      specialize (expr_only_ret' e σ1) as [n1 Hn1]. setoid_rewrite Hn1.
+      specialize (expr_only_ret' e σ2) as [n2 Hn2]. setoid_rewrite Hn2.
+      setoid_rewrite bind_ret_l. setoid_rewrite interp_state_trigger.
+      cbn. setoid_rewrite bind_trigger. apply pi_eqit_secure_priv_vislr; auto.
+      intros [] []. apply pi_eqit_secure_ret. split; auto.
+    + right; auto. unfold sem_stmt, interp_imp. intros σ1 σ2 Hσ.
+      cbn. setoid_rewrite interp_state_bind.
+      specialize (expr_only_ret' e σ1) as [n1 Hn1]. setoid_rewrite Hn1.
+      rewrite bind_ret_l. rewrite interp_state_trigger. cbn. rewrite bind_trigger.
+      apply pi_eqit_secure_priv_visl; auto. intros [].
+      apply pi_eqit_secure_ret. split; auto. cbv. auto.
+Qed.
+
+Lemma print_well_typed_correct' pc le lp e :
+  secure_expr le e -> leq (join le pc) lp ->
+  secure_throw_stmt pc Public (Output lp e).
+Proof.
+  intros He0 Hle1.
+  assert (Hle : leq le lp).
+  { eapply leq_sense_trans; eauto. apply leq_sense_join_l. }
+  assert (Hpc : leq pc lp).
+  { eapply leq_sense_trans; try apply H5. apply leq_sense_join_r; eauto. eauto.  }
+  assert (He : secure_expr lp e ).
+  { eapply secure_expr_upward_close with (l1 := le); eauto. }
+  intros observer. specialize (He observer).
+  inv He.
+  - left. eapply leq_sense_trans; eauto.
+    unfold sem_throw_stmt, interp_imp. intros σ1 σ2 Hσ.
+    cbn. setoid_rewrite throw_prefix_bind. setoid_rewrite interp_state_bind.
+    setoid_rewrite throw_prefix_denote_expr. setoid_rewrite interp_state_bind.
+    repeat rewrite bind_bind.
+    eapply pi_eqit_secure_bind; eauto.
+    intros [σ3 v1] [σ4 v4] [Hσ' Hv]; cbn in Hv; subst.
+    setoid_rewrite interp_state_ret. setoid_rewrite bind_ret_l.
+    cbn. setoid_rewrite throw_prefix_ev. setoid_rewrite interp_state_vis.
+    cbn. setoid_rewrite bind_trigger. setoid_rewrite bind_vis.
+    apply pi_eqit_secure_pub_vis; auto. intros [].
+    setoid_rewrite bind_ret_l. setoid_rewrite throw_prefix_ret.
+    tau_steps. apply pi_eqit_secure_ret. split; auto; constructor.
+  - case_leq pc observer.
+    + left; auto. unfold sem_throw_stmt, interp_imp. intros σ1 σ2 Hσ.
+      cbn. setoid_rewrite throw_prefix_bind.
+      setoid_rewrite throw_prefix_denote_expr. 
+      repeat setoid_rewrite interp_state_bind.
+      repeat rewrite bind_bind.
+      specialize (expr_only_ret' e σ1) as [n1 Hn1]. setoid_rewrite Hn1.
+      specialize (expr_only_ret' e σ2) as [n2 Hn2]. setoid_rewrite Hn2.
+      setoid_rewrite bind_ret_l.
+      setoid_rewrite interp_state_ret. setoid_rewrite bind_ret_l. cbn.
+      setoid_rewrite throw_prefix_ev.
+      setoid_rewrite interp_state_vis.
+      cbn. setoid_rewrite bind_trigger. 
+      setoid_rewrite bind_vis. 
+      apply pi_eqit_secure_priv_vislr; auto.
+      intros [] []. tau_steps. apply pi_eqit_secure_ret. split; auto. constructor.
+    + right; auto. unfold sem_throw_stmt, interp_imp. intros σ1 σ2 Hσ.
+      cbn. 
+      setoid_rewrite throw_prefix_bind. setoid_rewrite interp_state_bind.
+      setoid_rewrite throw_prefix_denote_expr.
+      setoid_rewrite interp_state_bind.
+      specialize (expr_only_ret' e σ1) as [n1 Hn1]. setoid_rewrite Hn1.
+      repeat rewrite bind_ret_l. 
+      rewrite interp_state_ret. rewrite bind_ret_l. cbn.
+      setoid_rewrite throw_prefix_ev.
+      rewrite interp_state_vis. cbn. rewrite bind_trigger.
+      rewrite bind_vis.
+      apply pi_eqit_secure_priv_visl; auto. intros [].
+      tau_steps.
+      apply pi_eqit_secure_ret. split; auto. cbv. constructor.
+Qed.
+
+Lemma skip_well_typed_correct pc :
+  secure_stmt pc Public Skip.
+Proof.
+  intros observer. case_leq pc observer.
+  - left; auto. do 2 red. unfold sem_stmt. intros σ1 σ2 Hσ.
+    cbn. setoid_rewrite interp_state_ret. apply pi_eqit_secure_ret.
+    split; auto.
+  - right; auto. do 2 red. unfold sem_stmt. intros σ1 σ2 Hσ.
+    cbn. setoid_rewrite interp_state_ret. apply pi_eqit_secure_ret.
+    split; auto. cbv. auto.
+Qed.
+
+Lemma skip_well_typed_correct' pc :
+  secure_throw_stmt pc Public Skip.
+Proof.
+  intros observer. case_leq pc observer.
+  - left; auto. do 2 red. unfold sem_throw_stmt. intros σ1 σ2 Hσ.
+    cbn. setoid_rewrite throw_prefix_ret.
+    setoid_rewrite interp_state_ret. apply pi_eqit_secure_ret.
+    split; auto. constructor.
+  - right; auto. do 2 red. unfold sem_throw_stmt. intros σ1 σ2 Hσ.
+    cbn. setoid_rewrite throw_prefix_ret.
+    setoid_rewrite interp_state_ret. apply pi_eqit_secure_ret.
+    split; auto. constructor.
+Qed.
+
+Lemma raise_well_typed pc lexn :
+  leq pc lexn -> secure_stmt pc lexn (Raise lexn).
+Proof.
+  intros Hpc observer. case_leq pc observer.
+  - left; auto. unfold sem_stmt, interp_imp. do 2 red. intros.
+    cbn. setoid_rewrite bind_trigger. setoid_rewrite interp_state_vis.
+    cbn. setoid_rewrite bind_trigger. setoid_rewrite bind_vis.
+    case_leq lexn observer.
+    + apply pi_eqit_secure_pub_vis. auto. intros [].
+    + apply pi_eqit_secure_priv_vislr; auto. intros [].
+  - right; auto. unfold sem_stmt, interp_imp. do 2 red. intros.
+    cbn. setoid_rewrite bind_trigger. setoid_rewrite interp_state_vis.
+    cbn. setoid_rewrite bind_trigger. setoid_rewrite bind_vis.
+    apply pi_eqit_secure_priv_visl. 2 : intros []. intro.
+    apply H. eapply leq_sense_trans; eauto.
+Qed.
+
+Lemma raise_well_typed' pc lexn :
+  leq pc lexn -> secure_throw_stmt pc lexn (Raise lexn).
+Proof.
+  intros Hpc observer. case_leq pc observer.
+  - left; auto. unfold sem_throw_stmt, interp_imp.
+    cbn. do 2 red. intros. setoid_rewrite bind_trigger.
+    setoid_rewrite throw_prefix_exc. setoid_rewrite interp_state_ret.
+    apply pi_eqit_secure_ret; auto. split; auto. constructor.
+    all : destruct lexn; cbv; auto.
+  - right; auto. do 2 red. intros. unfold sem_throw_stmt, interp_imp.
+    cbn. setoid_rewrite bind_trigger.
+    setoid_rewrite throw_prefix_exc. setoid_rewrite interp_state_ret.
+    apply pi_eqit_secure_ret. split; auto.
+    constructor. 2 : destruct lexn; cbv; auto. intro.
+    apply H. eapply leq_sense_trans; eauto.
+Qed.
+
+Definition well_typed_expr := SecurityImpTypes.well_typed_expr Γ.
 
 
 (* rework this definition to have only public exceptions*)
@@ -497,9 +990,47 @@ Inductive well_typed_stmt : sensitivity -> sensitivity -> stmt -> Prop :=
                            well_typed_stmt pc Public (Output lp e)
   | wts_if pc le e lexn1 lexn2 s1 s2 : well_typed_expr le e -> well_typed_stmt (join pc le) lexn1 s1 -> well_typed_stmt (join pc le) lexn2 s2 ->
                                        well_typed_stmt pc (join lexn1 lexn2) (If e s1 s2)
-  | wts_while e le pc lexn s : well_typed_expr le e -> well_typed_stmt (join pc le) lexn s ->
+  | wts_while e le pc lexn s : well_typed_expr le e -> well_typed_stmt (join pc (join le lexn)) lexn s ->
                          well_typed_stmt pc lexn (While e s)
   | wts_raise pc lexn : leq pc lexn -> well_typed_stmt pc lexn (Raise lexn)
   | wts_try pc lexn1 lexn2 s1 s2 : well_typed_stmt pc lexn1 s1 -> well_typed_stmt (join pc lexn1) lexn2 s2 ->
                                    well_typed_stmt pc lexn2 (TryCatch s1 s2)
 .
+
+Lemma well_typed_expr_correct e l : 
+  well_typed_expr l e -> secure_expr l e.
+Proof.
+  intros He observer.
+  apply well_typed_expr_correct in He.
+  specialize (He observer). inv He.
+  - left; auto. do 2 red. intros. eapply eqit_secure_imp_pi_eqit_scure; eauto.
+  - right; auto. destruct H0 as [n Hn]. exists n.
+    do 2 red. intros. eapply eqit_secure_imp_pi_eqit_scure; eauto.
+Qed.
+
+
+Lemma well_typed_stmt_sound s pc lexn : well_typed_stmt s pc lexn -> secure_stmt s pc lexn.
+Proof.
+  intros Htype. enough (secure_stmt s pc lexn /\ secure_throw_stmt s pc lexn); try tauto.
+  induction Htype; eauto.
+  - (* Skip *) split; try apply skip_well_typed_correct; try apply skip_well_typed_correct'.
+  - (* Seq *)
+    split; try apply seq_well_typed_correct; try apply seq_well_typed_correct'; tauto.
+  - (* Assign *)
+    split; try eapply assign_well_typed_correct; try eapply assign_well_typed_correct';
+      try apply well_typed_expr_correct; eauto.
+  - (* Output *)
+    split; try eapply print_well_typed_correct; try eapply print_well_typed_correct'; 
+      try apply well_typed_expr_correct; eauto.
+  - (* If *)
+    apply well_typed_expr_correct in H.
+    split; try eapply if_well_typed_correct; try eapply if_well_typed_correct'; eauto; try tauto.
+  - (* While *)
+    destruct IHHtype. apply well_typed_expr_correct in H.
+    split; try eapply while_well_typed_correct; try eapply while_well_typed_correct'; eauto.
+  - (* Raise *)
+    split; try eapply raise_well_typed; try eapply raise_well_typed'; eauto.
+  - (* TryCatch *)
+    destruct IHHtype1. destruct IHHtype2. 
+    split; try eapply try_catch_well_typed_correct; try eapply try_catch_well_typed_correct'; eauto.
+Qed.
