theories/Secure/SecurityImpExc/RaiseExceptionState.v
@@ -1,0 +1,130 @@
+From Coq Require Import
+     Arith.PeanoNat
+     Lists.List
+     Strings.String
+     Morphisms
+     Setoid
+     RelationClasses.
+
+From ExtLib Require Import
+     Data.String
+     Structures.Monad
+     Structures.Traversable
+     Data.List.
+
+From ITree Require Import
+     ITree
+     ITreeFacts
+     Events.MapDefault
+     Events.State
+     Events.StateFacts
+     Events.Exception
+     Events.ExceptionFacts
+     Core.Divergence
+     Dijkstra.TracesIT
+     Secure.SecureEqHalt
+     Secure.SecurityImpExc.SecurityImp
+     Secure.SecurityImpExc.SecurityImpHandlerExcState
+     Secure.SecureEqProgInsensEv
+.
+
+Import Monads.
+Import MonadNotation.
+Local Open Scope monad_scope.
+Local Open Scope string_scope.
+
+From Paco Require Import paco.
+
+
+Lemma interp_imp_try_catch R (ttry : itree _ R) kcatch σ:
+  interp_imp (try_catch ttry kcatch) σ ≈ 
+             try_catch (interp_imp ttry σ) (fun '(l, σ') => interp_imp (kcatch l) σ' ).
+Proof.
+  generalize dependent ttry. generalize dependent σ.
+  ginit. gcofix CIH. intros. 
+  destruct (observe ttry) eqn : Heq; symmetry in Heq; apply simpobs in Heq.
+  - setoid_rewrite Heq. setoid_rewrite try_catch_ret.
+    setoid_rewrite interp_state_ret. rewrite try_catch_ret.
+    gstep. constructor. auto.
+  - setoid_rewrite Heq.
+    rewrite try_catch_tau. setoid_rewrite interp_state_tau. rewrite try_catch_tau.
+    gstep. constructor. gfinal. left. eapply CIH.
+  - destruct e as [ ?  | [? | ? ] ].
+    + rewrite Heq. destruct e. rewrite try_catch_exc.
+      setoid_rewrite interp_state_vis. cbn.
+      repeat rewrite bind_trigger. rewrite bind_vis.
+      rewrite try_catch_exc. gfinal. right.
+      eapply paco2_mon with (r := bot2); intros; try contradiction.
+      enough (interp_imp (kcatch s) σ ≈ interp_imp (kcatch s) σ); auto.
+      reflexivity.
+    + rewrite Heq. destruct s.
+      * setoid_rewrite try_catch_ev. setoid_rewrite interp_state_vis.
+        cbn. setoid_rewrite bind_ret_l. rewrite try_catch_tau.
+        setoid_rewrite interp_state_tau. rewrite tau_euttge.
+        gstep. constructor. gfinal. left. eapply CIH.
+      * setoid_rewrite try_catch_ev. setoid_rewrite interp_state_vis.
+        cbn. setoid_rewrite bind_ret_l. rewrite try_catch_tau.
+        setoid_rewrite interp_state_tau. rewrite tau_euttge.
+        gstep. constructor. gfinal. left. eapply CIH.
+   + rewrite Heq. setoid_rewrite try_catch_ev. setoid_rewrite interp_state_vis.
+     cbn. repeat rewrite bind_trigger. repeat rewrite bind_vis. 
+     setoid_rewrite try_catch_ev. gstep. constructor.
+     intros. red. setoid_rewrite bind_ret_l. rewrite interp_state_tau.
+     rewrite try_catch_tau. gstep. constructor. gstep. constructor.
+     gfinal. left. eauto.
+Qed.
+
+
+(* what is the precise compositional condition 
+   maybe if I pick RE carefully there will be a clear compositional thing
+
+*)
+(* 
+Lemma interp_imp_try_catch_comp Label RE R RR ttry1 ttry2 kcatch1 kcatch2 :
+  (forall l1 l2 σ1 σ2, RE ... -> pi_eqit_secure Label  kcatch1 (l1, σ1) )
+*)
+
+(* this needs to take in two events can do tomorrow morning *)
+Variant Rexc (P : sensitivity -> map -> Prop) : forall A, (exceptE (sensitivity * map) +' IOE) A -> Prop :=
+  | rexcio A (io : IOE A) : Rexc P A (inr1 io) 
+  | rexc l σ : P l σ -> Rexc P void (inl1 (Throw _ (l, σ) ) )
+.
+
+(* Need something like the bind rule but for try_catch with the new pi_eqit_secure definition 
+   This is another trade off,
+   I am a bit worried about having space to talk about all of the differences and why we have
+   them, but that is what the meeting tomorrow is about 
+
+ *)
+
+(* Now I am concerned that my proposed new pi_eqit_secure is insufficient 
+   it constrains final states only in the case where both exceptions are public
+   I think I just need to talk with the rest of the team, figure out what to do
+
+   The key problem seems with the original proof lies with programs like this
+
+   while pub_x <> 0 do
+     x := x - 1;
+     if priv_y = 0 
+     then raise private 
+     else skip
+     print public pub_x
+   end
+
+   depending on initial value of priv_y it is either a sequence of prints to the
+   public stream or a single exception 
+
+   In the standard semantics this is fine
+   but when we interpret away exceptions,
+   this would enforce that a ret would be equiv to a print 
+
+
+   My original pi_eqit_secure definition still enables an improvement on the type system,
+   by relating spin to Ret, we can get a permissive while rule, even if we would still
+   need to be restrictive on the exceptions,
+   what I would need to do is change the Rsense relation, removing the mixed
+   cases and adding the restriction to public exceptions in the exception case 
+   the nice part is that this would only make the proofs easier
+
+   private exceptions are hard :`(
+ *)
