theories/Secure/SecurityImpExc/SecurityImpHandlerExcState.v
@@ -1,0 +1,52 @@
+From Coq Require Import
+     Arith.PeanoNat
+     Lists.List
+     Strings.String
+     Morphisms
+     Setoid
+     RelationClasses.
+
+From ExtLib Require Import
+     Data.String
+     Structures.Monad
+     Structures.Traversable
+     Data.List.
+
+From ITree Require Import
+     ITree
+     ITreeFacts
+     Events.MapDefault
+     Events.State
+     Events.StateFacts
+     Events.Exception
+     Core.Divergence
+     Dijkstra.TracesIT
+     Secure.SecureEqHalt
+     Secure.SecurityImpExc.SecurityImp
+.
+
+
+Import Monads.
+Import MonadNotation.
+Local Open Scope monad_scope.
+Local Open Scope string_scope.
+
+From Paco Require Import paco.
+
+
+Definition handle_state_io {E} : forall A, (stateE +' IOE) A -> stateT map (itree (E +' IOE)) A :=
+  fun _ e => match e with
+          | inl1 el => handleState _ el
+          | inr1 er => fun s => r <- ITree.trigger (inr1 er);; Ret (s, r) end. 
+
+Definition handle_exc :forall A, exceptE sensitivity A -> stateT map  (itree ((exceptE (sensitivity * map))  +' IOE) ) A :=
+  fun _ e => match e with
+            | Throw _ l => fun s => r <- ITree.trigger (inl1 (Throw _ (l, s) ) );; Ret (s, r) end.
+
+Program Definition handle_imp_exc : forall A, ((exceptE sensitivity) +' stateE +' IOE) A -> stateT map (itree ((exceptE (sensitivity * map))  +' IOE) ) A :=
+  fun _ e => match e with
+          | inl1 exc => handle_exc _ exc
+          | inr1 er => handle_state_io _ er end.
+
+Definition interp_imp {R} (t : itree (impExcE +' stateE +' IOE) R ) : stateT map (itree (exceptE (sensitivity * map) +' IOE)) R :=
+  interp_state handle_imp_exc t. 
